Prove CountDownLatch

formal-proofs/theories/lib/barrier/barrier.v
@@ -2,6 +2,7 @@ Require Import SegmentQueue.lib.thread_queue.thread_queue.
 From SegmentQueue.lib.concurrent_linked_list.infinite_array
      Require Import array_spec iterator.iterator_impl.
 Require Import SegmentQueue.lib.util.future.
+Require Import SegmentQueue.lib.util.forRange.
 From iris.heap_lang Require Import notation.
 
 Section impl.
@@ -11,12 +12,6 @@ Variable limit: positive.
 
 Definition newBarrier: val :=
   λ: <>, (ref #0, newThreadQueue array_interface #()).
-
-Definition forRange : val :=
-  rec: "loop" "n" "fn" :=
-    if: "n" ≤ #0
-    then #()
-    else "loop" ("n"-#1) "fn" ;; "fn" ("n"-#1).
 
 Definition barrierResume: val :=
   λ: "d", resume array_interface #(Z.of_nat 300) #true #false #false "d"
@@ -58,65 +53,6 @@ From iris.base_logic.lib Require Import invariants.
 From iris.algebra Require Import numbers auth list gset excl csum.
 From iris.program_logic Require Import atomic.
 From iris.heap_lang Require Import proofmode.
-
-Section for_proof.
-
-Context `{!heapG Σ}.
-
-Theorem forRange_spec (Φ: nat -> iProp Σ) (e: val) (n: nat):
-  (∀ i, ⌜(i < n)%nat⌝ -∗ {{{ Φ i }}}
-                           e #i
-                         {{{ v, RET v; Φ (S i) }}})
-   -∗
-   {{{ Φ O }}}
-     forRange #n e
-   {{{ v, RET v; Φ n }}}.
-Proof.
-  iIntros "#HE" (Ψ).
-  iInduction n as [|n'] "IH" forall (Ψ); iIntros "!> HΦ0 HΨ"; wp_lam; wp_pures.
-  by iApply "HΨ".
-  replace #(S n' - 1) with #n'; last by congr (fun x => LitV (LitInt x)); lia.
-  wp_bind (forRange _ _).
-  wp_apply ("IH" with "[] HΦ0").
-  { iIntros "!>" (i HLt). iApply "HE". iPureIntro. lia. }
-  iIntros (v) "HΦn".
-  wp_pures.
-  replace #(S n' - 1) with #n'; last by congr (fun x => LitV (LitInt x)); lia.
-  wp_apply ("HE" with "[] HΦn"); last done.
-  iPureIntro. lia.
-Qed.
-
-Theorem forRange_resource_map (Φ Ψ: nat -> iProp Σ) (e: val):
-  (∀ (i: nat), {{{ Φ i }}}
-                 e #i
-                 {{{ v, RET v; Ψ i }}})
-    -∗
-  (∀ n, {{{ [∗ list] i ∈ seq 0 n, Φ i }}}
-          forRange #n e
-        {{{ v, RET v; [∗ list] i ∈ seq 0 n, Ψ i }}}).
-Proof.
-  iIntros "#HE" (n Ξ) "!> HΦ HΨ".
-  iApply (forRange_spec
-            (fun j => ([∗ list] i ∈ seq j (n-j), Φ i) ∗
-                   ([∗ list] i ∈ seq 0 j, Ψ i))%I
-            with "[] [HΦ]").
-  - iIntros (i HLt). iIntros "!>" (?) "HPre HPost".
-    replace (seq 0 (S i)) with (seq 0 (i + 1)) by (congr (seq 0); lia).
-    rewrite seq_add /=.
-    destruct (n - i)%nat as [|ni] eqn:X; first by lia.
-    simpl.
-    iDestruct "HPre" as "[[HΦi HΦ] HΨ]".
-    wp_apply ("HE" with "HΦi").
-    iIntros (v) "HΨi".
-    iApply "HPost".
-    replace (n - S i)%nat with ni by lia. iFrame. done.
-  - rewrite Nat.sub_0_r. simpl. iFrame.
-  - iIntros (v) "!> HH".
-    iApply "HΨ".
-    iDestruct "HH" as "[_ $]".
-Qed.
-
-End for_proof.
 
 Section proof.
 
@@ -313,7 +249,8 @@ Proof.
     + by rewrite -big_sepL_replicate seq_length.
     + iIntros (?) "_". wp_pures.
       iApply (fillThreadQueueFuture_spec with "[HMyExit]").
-      2: { iIntros "!>" (γf v') "H". iApply "HΦ". iFrame "HInhabit H". }
+      2: { iIntros "!>" (γf v') "(H1 & H2 & _)". iApply "HΦ".
+           iFrame "HInhabit H1 H2". }
       rewrite /V'. simpl. iExists _. iFrame. by iPureIntro.
   - iMod (thread_queue_append' with "HTq [] HState")
       as "[HState HSus]"=> /=; [by solve_ndisj|done|].
