formal-proofs/theories/lib/countdownlatch/countdownlatch.v
@@ -1,0 +1,654 @@
+Require Import SegmentQueue.lib.thread_queue.thread_queue.
+From SegmentQueue.lib.concurrent_linked_list.infinite_array
+     Require Import array_spec iterator.iterator_impl.
+From SegmentQueue.lib.util Require Import future getAndUpdate forRange.
+From iris.heap_lang Require Import notation.
+
+Section impl.
+
+Variable array_interface: infiniteArrayInterface.
+
+Definition newLatch: val :=
+  λ: "count", (ref "count", ref #0, newThreadQueue array_interface #()).
+
+Definition latchResume: val :=
+  λ: "d", resume array_interface #(Z.of_nat 300) #true #false #false "d"
+                 (λ: <>, #()) #().
+
+(* Differs from the canonical implementation to be able to ignore the size of the
+   memory cell. *)
+Definition addWaiter: val := λ: "waiters", FAA "waiters" #2.
+Definition removeWaiter: val := λ: "waiters", FAA "waiters" #(-2).
+Definition hasDoneMark: val := λ: "w", "w" `rem` #2 = #1.
+Definition setDoneMark: val := λ: "w", "w" + #1.
+
+Definition resumeWaiters: val :=
+  λ: "latch",
+  let: "waiters" := Snd (Fst "latch") in
+  let: "d" := Snd (Snd "latch") in
+  let: "w" := getAndUpdate
+                "waiters"
+                (λ: "cur",
+                 if: hasDoneMark "cur"
+                 then NONE
+                 else SOME (setDoneMark "cur"))
+  in match: "w" with
+        NONE => #()
+      | SOME "w'" => forRange ("w'" `quot` #2) (λ: <>, latchResume "d");; #()
+     end.
+
+Definition countDown: val :=
+  λ: "latch",
+  let: "counter" := Fst (Fst "latch") in
+  let: "d" := Snd (Snd "latch") in
+  let: "p" := FAA "counter" #(-1) in
+  if: "p" - #1 ≤ #0 then resumeWaiters "latch" else #().
+
+Definition await: val :=
+  λ: "latch",
+  let: "counter" := Fst (Fst "latch") in
+  let: "waiters" := Snd (Fst "latch") in
+  let: "e" := Fst (Snd "latch") in
+  if: !"counter" ≤ #0 then fillThreadQueueFuture #()
+  else let: "w" := addWaiter "waiters" in
+       if: hasDoneMark "w" then fillThreadQueueFuture #()
+       else match: suspend array_interface "e" with
+              InjR "f" => "f"
+            | InjL "x" => "undefined"
+            end.
+
+Definition cancelLatchFuture : val :=
+  λ: "latch" "f",
+  let: "waiters" := Snd (Fst "latch") in
+  let: "onCancellation" :=
+     λ: <>, let: "w" := removeWaiter "waiters" in ~ (hasDoneMark "w")
+  in
+  let: "d" := Snd (Snd "latch") in
+  tryCancelThreadQueueFuture' array_interface
+                              #false #(Z.of_nat 300) #false #false
+                              "d" "onCancellation"
+                              (λ: <>, #()) (λ: <>, #()) "f".
+
+Definition getCount: val :=
+  λ: "latch",
+  let: "counter" := Fst (Fst "latch") in
+  let: "c" := !"counter" in
+  if: "c" ≤ #0 then #0 else "c".
+
+End impl.
+
+From SegmentQueue.util Require Import everything big_opL local_updates.
+From iris.base_logic.lib Require Import invariants.
+From iris.algebra Require Import numbers auth list gset excl csum.
+From iris.program_logic Require Import atomic.
+From iris.heap_lang Require Import proofmode.
+
+Section proof.
+
+Notation algebra := (authR (prodUR
+                              natUR
+                              (optionUR (csumR (exclR positiveR)
+                                                (optionR (agreeR unitO)))))).
+
+Class latchG Σ := BarrierG { barrier_inG :> inG Σ algebra }.
+Definition latchΣ : gFunctors := #[GFunctor algebra].
+Instance subG_latchΣ {Σ} : subG latchΣ Σ -> latchG Σ.
+Proof. solve_inG. Qed.
+
+Context `{heapG Σ} `{iteratorG Σ} `{threadQueueG Σ} `{futureG Σ} `{latchG Σ}.
+Variable (N NFuture: namespace).
+Variable (HNDisj: N ## NFuture).
+Let NLatch := N .@ "Latch".
+Let NTq := N .@ "Tq".
+Notation iProp := (iProp Σ).
+
+Variable array_interface: infiniteArrayInterface.
+Variable array_spec: infiniteArraySpec _ array_interface.
+
+Definition latch_broken γ := own γ (◯ (0, Some (Cinr ε))).
+
+Definition latch_closed γ := own γ (◯ (0, Some (Cinr (Some (to_agree ()))))).
+
+Definition latch_waiter_registered γ := own γ (◯ (1, ε)).
+
+Definition latch_waiter_permit γ γf: iProp :=
+  latch_waiter_registered γ ∨
+  (∃ v, future_is_completed γf v).
+
+Global Instance latch_broken_persistent: Persistent (latch_broken γ).
+Proof. apply _. Qed.
+
+Let tqParams γl :=
+  @ThreadQueueParameters Σ false True (latch_broken γl) True
+                         (fun v => ⌜#v = #()⌝)%I False.
+
+Let isThreadQueue γl := is_thread_queue NTq NFuture (tqParams γl) _ array_spec.
+
+Definition is_latch_future γl :=
+  is_thread_queue_future NTq NFuture (tqParams γl) _ array_spec.
+
+Lemma resumeLatch_spec R maxWait (wait: bool) γa γtq γe γd e d:
+  {{{ isThreadQueue R γa γtq γe γd e d ∗ awakening_permit γtq }}}
+    resume array_interface #(Z.of_nat maxWait) #true #false #wait d (λ: <>, #())%V #()
+  {{{ RET #true; True }}}.
+Proof.
+  iIntros (Φ) "[#HTq HAwak] HΦ".
+  iApply (resume_spec with "[] [HAwak]").
+  5: { by iFrame "HTq HAwak". }
+  by solve_ndisj. done. done.
+  { simpl. iIntros (Ψ) "!> _ HΨ". wp_pures. by iApply "HΨ". }
+  iIntros "!>" (r) "Hr". simpl. destruct r; first by iApply "HΦ".
+  iDestruct "Hr" as "[% _]"; lia.
+Qed.
+
+Definition latch_invariant (γl γtq: gname) (ℓ wℓ: loc) (n: nat) (w: nat): iProp :=
+  wℓ ↦ #(w * 2)%nat ∗ thread_queue_state γtq w ∗
+    (⌜n > 0⌝ ∧ own γl (● (w, Some (Cinl (Excl (Pos.of_nat n))))) ∗ ℓ ↦ #n ∨
+     ⌜n = 0⌝ ∧ own γl (● (w, Some (Cinr None))) ∗
+        (∃ n', ⌜(n' ≤ 0)%Z⌝ ∧ ℓ ↦ #n')) ∨
+  wℓ ↦ #(w * 2 + 1)%nat ∗ thread_queue_state γtq 0 ∗
+    ⌜n = 0⌝ ∗ own γl (● (w, Some (Cinr (Some (to_agree ()))))) ∗
+    (∃ n', ⌜(n' ≤ 0)%Z⌝ ∧ ℓ ↦ #n').
+
+Definition is_latch γl γa γtq γe γd (s: val): iProp :=
+  ∃ e d (p pw: loc), ⌜s = (#p, #pw, (e, d))%V⌝ ∧
+  inv NLatch (∃ n w, latch_invariant γl γtq p pw n w)
+  ∗ isThreadQueue γl γa γtq γe γd e d.
+
+Definition latch_state γl (counter: nat): iProp :=
+  own γl (◯ (0, Some (match counter with
+        0 => Cinr ε
+      | _ => Cinl (Excl (Pos.of_nat counter))
+                      end))).
+
+Theorem newLatch_spec (n: nat):
+  n > 0 ->
+  {{{ inv_heap_inv }}}
+    newLatch array_interface #n
+  {{{ γl γa γtq γe γd s, RET s; is_latch γl γa γtq γe γd s ∗
+                                         latch_state γl n
+  }}}.
+Proof.
+  iIntros (Hn Φ) "#HHeap HΦ".
+  iMod (own_alloc (● (0, Some (Cinl (Excl (Pos.of_nat n)))) ⋅
+                   ◯ (0, Some (Cinl (Excl (Pos.of_nat n))))))
+    as (γl) "[H● H◯]".
+  by apply auth_both_valid=> //.
+  wp_lam. wp_bind (newThreadQueue _ _).
+  iApply (newThreadQueue_spec with "HHeap").
+  iIntros (γa γtq γe γd e d) "!> [#HTq HThreadState]".
+  wp_alloc pw as "Hpw". wp_alloc p as "Hp". rewrite -wp_fupd. wp_pures.
+  iMod (inv_alloc NLatch _ (∃ n w, latch_invariant γl γtq p pw n w) with "[-HΦ H◯]")
+    as "#HInv".
+  { iExists n, 0. simpl. iLeft. iFrame "Hpw HThreadState". iLeft. iFrame.
+    by iPureIntro. }
+  iApply "HΦ". iSplitR.
+  { iExists _, _, _, _. iSplitR; first done. by iFrame "HInv HTq". }
+  rewrite /latch_state. by destruct n; first lia.
+Qed.
+
+Lemma await_spec γl γa γtq γe γd s:
+  {{{ is_latch γl γa γtq γe γd s }}}
+    await array_interface s @ ⊤
+  {{{ γf v, RET v;
+      is_latch_future γl γtq γa γf v ∗
+      thread_queue_future_cancellation_permit γf ∗
+      latch_waiter_permit γl γf }}}.
+Proof.
+  iIntros (Φ) "#HLatch HΦ". wp_lam. rewrite /is_latch.
+  iDestruct "HLatch" as (e d p pw ->) "[HInv HTq]".
+  wp_pures. wp_bind (!_)%E.
+  iInv "HInv" as (n w) "HLatchInv" "HClose".
+  iDestruct "HLatchInv" as
+      "[(Hpw & HTqState & [(>% & H● & Hp)|(>-> & H● & Hp)])|
+        (Hpw & HTqState & >-> & H● & Hp)]".
+  - wp_load. iMod ("HClose" with "[-HΦ]") as "_".
+    { iExists _, _. iLeft. iFrame "Hpw HTqState". iLeft. by iFrame. }
+    iModIntro. wp_pures. rewrite bool_decide_false; last lia. clear. wp_pures.
+    wp_lam. wp_bind (FAA _ _).
+    iInv "HInv" as (n w) "HLatchInv" "HClose".
+    iDestruct "HLatchInv" as "[(Hpw & HTqState & HRest)|
+      (Hpw & HTqState & >-> & H● & Hp)]".
+    * wp_faa.
+      iMod (thread_queue_append' with "HTq [] HTqState")
+        as "[HState HSus]"=> /=; [by solve_ndisj|done|].
+      iAssert (
+          |==>
+          latch_waiter_registered γl ∗
+          (⌜n > 0⌝ ∧ own γl (● (S w, Some (Cinl (Excl (Pos.of_nat n))))) ∗ p ↦ #n
+           ∨ ⌜n = 0⌝ ∧ own γl (● (S w, Some (Cinr None))) ∗ (∃ n' : Z, ⌜(n' ≤ 0)%Z⌝ ∧ p ↦ #n'))
+      )%I with "[HRest]" as ">[HToken HRest]".
+      {
+        iDestruct "HRest" as "[(H1 & H● & H2)|(H1 & H● & H2)]".
+        2: iMod (own_update with "H●") as "[H● $]"; last by iRight; iFrame.
+        1: iMod (own_update with "H●") as "[H● $]"; last by iLeft; iFrame.
+        all: apply auth_update_alloc, prod_local_update_1, nat_local_update.
+        all: replace ε with 0 by done; lia.
+      }
+      iMod ("HClose" with "[-HSus HΦ HToken]") as "_".
+      { iExists _, _. iLeft. iFrame.
+        replace ((w * 2)%nat + 2)%Z with (Z.of_nat (S w * 2)) by lia.
+        by iFrame. }
+      iModIntro. wp_pures. wp_lam. wp_pures. rewrite bool_decide_false.
+      2: { case. rewrite Nat2Z.inj_mul Z.rem_mul; lia. }
+      wp_pures. wp_apply (suspend_spec with "[$]")=>/=.
+      iIntros (v) "[(_ & _ & %)|Hv]"; first done.
+      iDestruct "Hv" as (γf v' ->) "[HFuture HCancPermit]".
+      wp_pures. iApply "HΦ". iFrame.
+    * wp_faa.
+      iAssert (|==> own γl (● (S w, Some (Cinr _))) ∗
+                    (latch_broken γl ∗ latch_waiter_registered γl))%I
+        with "[H●]" as ">[H● [H◯ HToken]]".
+      { iMod (own_update with "H●") as "[$ [$ $]]"; last done.
+        apply auth_update_alloc=> /=. apply prod_local_update=> /=.
+        - apply nat_local_update. replace ε with 0 by done.
+          replace (0 ⋅ 1) with 1 by done. lia.
+        - rewrite cmra_comm. apply core_id_local_update.
+          apply _. apply Some_included. right. apply Cinr_included.
+          apply ucmra_unit_least.
+      }
+      iMod ("HClose" with "[-HΦ H◯ HToken]") as "_".
+      { iExists 0, (S w). iRight. iFrame. iSplitL; last done.
+        by replace (Z.of_nat (S w * 2 + 1)) with ((w * 2 + 1)%nat + 2)%Z by lia. }
+      iModIntro. wp_pures. wp_lam. wp_pures. rewrite bool_decide_true.
+      2: { congr LitV.
+        rewrite Nat.add_comm Nat2Z.inj_add Nat2Z.inj_mul Z.rem_add //; lia. }
+      wp_pures.
+      iApply (fillThreadQueueFuture_spec with "[H◯]").
+      2: by iIntros "!>" (γf v') "(H & H' & H'')"; iApply "HΦ"; iFrame.
+      rewrite /V'. iExists _. simpl. iFrame. done.
+  - iDestruct "Hp" as (n') "[>% Hp]". wp_load.
+    iAssert (|==> own γl (● _) ∗ latch_broken γl)%I with "[H●]" as ">[H● H◯]".
+    { iMod (own_update with "H●") as "[$ $]"; last done.
+      apply auth_update_core_id. apply _. apply prod_included=> /=. split.
+      by apply nat_included; lia.
+      apply Some_included. right. apply Cinr_included. apply ucmra_unit_least. }
+    iMod ("HClose" with "[-HΦ H◯]") as "_".
+    { iExists _, _. iLeft. iFrame "Hpw HTqState". iRight. iFrame.
+      iSplitR; first done. iExists n'. iFrame. done. }
+    iModIntro. wp_pures. rewrite bool_decide_true; last lia. wp_pures.
+    iApply (fillThreadQueueFuture_spec with "[H◯]").
+    2: { iIntros "!>" (γf v') "(H & H' & H'')"; iApply "HΦ"; iFrame.
+         by iRight; iExists _. }
+    rewrite /V'. iExists _. simpl. iFrame. done.
+  - iDestruct "Hp" as (n') "[>% Hp]". wp_load.
+    iAssert (|==> own γl (● _) ∗ latch_broken γl)%I with "[H●]" as ">[H● H◯]".
+    { iMod (own_update with "H●") as "[$ $]"; last done.
+      apply auth_update_core_id. apply _. apply prod_included=> /=. split.
+      by apply nat_included; lia.
+      apply Some_included. right. apply Cinr_included. apply ucmra_unit_least. }
+    iMod ("HClose" with "[-HΦ H◯]") as "_".
+    { iExists _, _. iRight. iFrame "Hpw HTqState". iFrame.
+      iSplitR; first done. iExists n'. iFrame. done. }
+    iModIntro. wp_pures. rewrite bool_decide_true; last lia. wp_pures.
+    iApply (fillThreadQueueFuture_spec with "[H◯]").
+    2: {
+      iIntros "!>" (γf v') "(H & H' & H'')"; iApply "HΦ"; iFrame.
+      iRight. by iExists _. }
+    rewrite /V'. iExists _. simpl. iFrame. done.
+Qed.
+
+Lemma excl_included {A: ofeT} (a b: A): Excl a ≼ Excl b -> a ≡ b.
+Proof. intros [x y]. destruct x; inversion_clear y. Qed.
+
+Lemma getCount_spec γl γa γtq γe γd s:
+  is_latch γl γa γtq γe γd s -∗
+  <<< ∀ (n: nat), latch_state γl n >>>
+    getCount s @ ⊤ ∖ ↑NLatch
+  <<< latch_state γl n, RET #n >>>.
+Proof.
+  iIntros "#HLatch" (Φ) "AU". wp_lam.
+  iDestruct "HLatch" as (e d p pw ->) "[HInv HTq]". wp_pures. wp_bind (!_)%E.
+  iInv "HInv" as (n' w) "HOpen" "HInvClose".
+  iMod "AU" as (n) "[HState [_ HClose]]".
+  iDestruct "HOpen" as
+      "[(Hpw & HTqState & [(>% & H● & Hp)|(>-> & H● & Hp)])|
+        (Hpw & HTqState & >-> & H● & Hp)]".
+  - wp_load.
+    iAssert (⌜n' = n⌝)%I as %->.
+    { iDestruct (own_valid_2 with "H● HState")
+        as %[[_ HValid%Some_included]%prod_included _]%auth_both_valid.
+      destruct n as [|n].
+      { exfalso. move: HValid. case. by move=> HContra; inversion HContra.
+        rewrite csum_included. case; first done.
+        case; intros (? & ? & ? & ? & ?)=> //. }
+      iPureIntro. move: HValid. rewrite Cinl_included.
+      case; move=> HValid; [apply Cinl_inj in HValid; inversion HValid; subst|
+                           apply excl_included in HValid].
+      all: apply Nat2Pos.inj; [lia|lia|done].
+    }
+    iMod ("HClose" with "HState") as "HΦ". iModIntro.
+    iMod ("HInvClose" with "[-HΦ]") as "_".
+    { iExists _, _. iLeft. iFrame "Hpw HTqState". iLeft. by iFrame. }
+    iModIntro. wp_pures. rewrite bool_decide_false; last lia. by wp_pures.
+  - iDestruct "Hp" as (n'') "[>% Hp]".
+    wp_load.
+    iAssert (⌜n = 0⌝)%I as %->.
+    { iDestruct (own_valid_2 with "H● HState")
+        as %[[_ HValid%Some_included]%prod_included _]%auth_both_valid.
+      destruct n as [|n]; first done.
+      { exfalso. move: HValid. case. by move=> HContra; inversion HContra.
+        rewrite csum_included. case; first done.
+        case; intros (? & ? & ? & ? & ?)=> //. }
+    }
+    iMod ("HClose" with "HState") as "HΦ". iModIntro.
+    iMod ("HInvClose" with "[-HΦ]") as "_".
+    { iExists _, _. iLeft. iFrame "Hpw HTqState". iRight. iFrame.
+      iSplitR; first done. iExists _. iSplitR; last iFrame. done. }
+    iModIntro. wp_pures. rewrite bool_decide_true; last lia.
+    by wp_pures.
+  - iDestruct "Hp" as (n'') "[>% Hp]".
+    wp_load.
+    iAssert (⌜n = 0⌝)%I as %->.
+    { iDestruct (own_valid_2 with "H● HState")
+        as %[[_ HValid%Some_included]%prod_included _]%auth_both_valid.
+      destruct n as [|n]; first done.
+      { exfalso. move: HValid. case. by move=> HContra; inversion HContra.
+        rewrite csum_included. case; first done.
+        case; intros (? & ? & ? & ? & ?)=> //. }
+    }
+    iMod ("HClose" with "HState") as "HΦ". iModIntro.
+    iMod ("HInvClose" with "[-HΦ]") as "_".
+    { iExists _, _. iRight. iFrame.
+      iSplitR; first done. iExists _. iSplitR; last iFrame. done. }
+    iModIntro. wp_pures. rewrite bool_decide_true; last lia.
+    by wp_pures.
+Qed.
+
+Lemma resumeWaiters_spec γl γa γtq γe γd s:
+  {{{ is_latch γl γa γtq γe γd s ∗ latch_broken γl }}}
+    resumeWaiters array_interface s
+  {{{ RET #(); True }}}.
+Proof.
+  iIntros (Φ) "[#HLatch #HBroken] HΦ". wp_lam.
+  iDestruct "HLatch" as (e d p pw ->) "[HInv HTq]". wp_pures.
+  wp_lam. wp_pures.
+  iLöb as "IH".
+  wp_bind (!_)%E.
+  iInv "HInv" as (n w) "HLatchInv" "HClose".
+  iDestruct "HLatchInv" as
+      "[(Hpw & HTqState & HRest)|
+        (Hpw & HTqState & >-> & H● & Hp)]".
+  all: wp_load.
+  - iMod ("HClose" with "[-HΦ]") as "_".
+    { iExists _, _. iLeft. iFrame "Hpw HTqState". by iFrame. }
+    iModIntro. wp_pures. wp_lam. wp_pures. rewrite bool_decide_false.
+    2: { case. rewrite Nat2Z.inj_mul Z.rem_mul; lia. }
+    wp_pures. wp_lam. wp_pures. wp_bind (CmpXchg _ _ _). clear n.
+    iInv "HInv" as (n w') "HLatchInv" "HClose".
+    iDestruct "HLatchInv" as
+        "[(Hpw & HTqState & HRest)|(Hpw & HTqState & >-> & H● & Hp)]".
+    2: { wp_cmpxchg_fail. case; lia.
+         iMod ("HClose" with "[-HΦ]") as "_".
+         { iExists _, _. iRight. by iFrame. }
+         iModIntro. wp_pures. wp_lam. wp_pures. by iApply "IH". }
+    destruct (decide (w = w')).
+    2: { wp_cmpxchg_fail. case; lia.
+         iMod ("HClose" with "[-HΦ]") as "_".
+         { iExists _, _. iLeft. by iFrame. }
+         iModIntro. wp_pures. wp_lam. wp_pures. by iApply "IH". }
+    wp_cmpxchg_suc. subst w'.
+    iAssert (|={⊤ ∖ ↑NLatch}=> thread_queue_state γtq 0 ∗
+            [∗] replicate w (awakening_permit γtq))%I
+      with "[HTqState]" as ">[HState HAwaks]".
+    {
+      iClear "IH". clear. iInduction (w) as [|w] "IH"=>/=. by iFrame.
+      iMod (thread_queue_register_for_dequeue' with
+                "HTq [$] [$]") as "[HState $]". by solve_ndisj.
+      lia. rewrite /= Nat.sub_0_r.
+      iApply ("IH" with "HState").
+    }
+    iDestruct "HRest" as "[(_ & HContra & _)|(-> & H● & Hp)]".
+    { iDestruct (own_valid_2 with "HContra HBroken")
+        as %[[_ HValid]%prod_included _]%auth_both_valid.
+      exfalso. move: HValid. rewrite Some_included. case.
+      by intros HValid; inversion HValid.
+      rewrite csum_included. case; first done.
+      case; by intros (? & ? & ? & ? & ?). }
+    iAssert (|==> own γl _ ∗ latch_closed γl)%I with "[H●]" as ">[H● H◯]".
+    2: iMod ("HClose" with "[-HΦ H◯ HAwaks]") as "_".
+    2: {
+      iExists _, w. iRight. iFrame "HState". iSplitL "Hpw".
+      by rewrite Nat2Z.inj_add.
+      iSplitR; first done. iFrame.
+    }
+    { iMod (own_update with "H●") as "[$ $]"; last done.
+      apply auth_update_alloc, prod_local_update_2, option_local_update'''=> //. }
+    iModIntro. wp_pures. replace 2%Z with (Z.of_nat 2) by lia.
+    rewrite quot_of_nat Nat.div_mul; last lia.
+    wp_apply (forRange_resource_map
+                (fun _ => awakening_permit γtq) (fun _ => True)%I
+             with "[] [HAwaks]").
+    + iIntros (i Ψ) "!> HAwak HΨ". wp_pures. wp_lam.
+      wp_apply (resumeLatch_spec with "[$]"). iIntros (_).
+      by iApply "HΨ".
+    + by rewrite -big_sepL_replicate seq_length.
+    + iIntros (?) "_". wp_pures. by iApply "HΦ".
+  - iMod ("HClose" with "[-HΦ]") as "_".
+    { iExists _, _. iRight. by iFrame. }
+    iModIntro. wp_pures. wp_lam. wp_pures. rewrite bool_decide_true.
+    2: { congr LitV.
+         rewrite Nat.add_comm Nat2Z.inj_add Nat2Z.inj_mul Z.rem_add //; lia. }
+    wp_pures. by iApply "HΦ".
+Qed.
+
+Lemma countDown_spec γl γa γtq γe γd s:
+  is_latch γl γa γtq γe γd s -∗
+  <<< ∀ n, latch_state γl n >>>
+    countDown array_interface s @ ⊤ ∖ ↑NLatch
+  <<< if decide (2 ≤ n)%nat then latch_state γl (n - 1)
+      else latch_state γl 0 ∗ latch_broken γl,
+      RET #() >>>.
+Proof.
+  iIntros "#HLatch" (Φ) "AU". wp_lam.
+  iDestruct "HLatch" as (e d p pw ->) "[HInv HTq]". wp_pures. wp_bind (FAA _ _).
+  iInv "HInv" as (n' w) "HOpen" "HInvClose".
+  iMod "AU" as (n) "[HState [_ HClose]]".
+  iDestruct "HOpen" as
+      "[(Hpw & HTqState & [(>% & H● & Hp)|(>-> & H● & Hp)])|
+        (Hpw & HTqState & >-> & H● & Hp)]".
+  - wp_faa.
+    iAssert (⌜n' = n⌝)%I as %->.
+    { iDestruct (own_valid_2 with "H● HState")
+        as %[[_ HValid%Some_included]%prod_included _]%auth_both_valid.
+      destruct n as [|n].
+      { exfalso. move: HValid. case. by move=> HContra; inversion HContra.
+        rewrite csum_included. case; first done.
+        case; intros (? & ? & ? & ? & ?)=> //. }
+      iPureIntro. move: HValid. rewrite Cinl_included.
+      case; move=> HValid; [apply Cinl_inj in HValid; inversion HValid; subst|
+                           apply excl_included in HValid].
+      all: apply Nat2Pos.inj; [lia|lia|done].
+    }
+    destruct (decide (2 ≤ n)).
+    * rewrite /latch_state. destruct n as [|[|rn]]; [lia | lia |]. simpl.
+      iAssert (|==> own γl (● (w, Some (Cinl (Excl (Pos.of_nat (S rn))))))
+                    ∗ own γl (◯ (0, Some (Cinl (Excl (Pos.of_nat (S rn)))))))%I
+              with "[H● HState]" as ">[H● HState]".
+      { iDestruct (own_update_2 with "H● HState") as ">[$ $]"; last done.
+        apply auth_update, prod_local_update_2, option_local_update, csum_local_update_l=> /=.
+        by apply exclusive_local_update. }
+      iMod ("HClose" with "HState") as "HΦ". iModIntro.
+      iMod ("HInvClose" with "[-HΦ]") as "_".
+      { iExists _, _. iLeft. iFrame "Hpw HTqState". iLeft. iFrame "H●".
+        iSplitR; first by iPureIntro; lia.
+        by replace (Z.of_nat (S rn)) with ((2 + rn)%nat + -1)%Z by lia. }
+      iModIntro. wp_pures. rewrite bool_decide_false; last by lia. by wp_pures.
+    * rewrite /latch_state. destruct n as [|[|]]; last lia.
+      { iDestruct (own_valid_2 with "H● HState")
+          as %[[_ HValid%Some_included]%prod_included _]%auth_both_valid. exfalso.
+        move: HValid; case=> HValid. by inversion HValid.
+        move: HValid. rewrite csum_included.
+        case; first done. case; intros (? & ? & ? & ? & ?)=> //. }
+      iAssert (|==> own γl (● (w, Some (Cinr ε))) ∗ own γl (◯ (0, Some (Cinr ε))))%I
+              with "[H● HState]" as ">[H● #HState]".
+      { iMod (own_update_2 with "H● HState") as "[$ $]"; last done.
+        apply auth_update, prod_local_update_2.
+        etransitivity. by apply delete_option_local_update, _.
+        apply alloc_option_local_update. done. }
+      iMod ("HClose" with "[$]") as "HΦ". iModIntro.
+      iMod ("HInvClose" with "[-HΦ]") as "_".
+      { iExists 0, _. iLeft. iFrame "Hpw HTqState". iRight. iFrame.
+        iSplitR; first done. iExists 0. by iFrame. }
+      iModIntro. wp_pures.
+      wp_apply resumeWaiters_spec.
+      { iFrame "HState". iExists _, _, _, _. iSplitR; first done.
+        iFrame "HInv HTq". }
+      by iIntros "_".
+  - iDestruct "Hp" as (n') "[>% Hp]". wp_faa.
+    destruct n=>/=.
+    2: {
+      iDestruct (own_valid_2 with "H● HState")
+        as %[[_ HValid%Some_included]%prod_included _]%auth_both_valid.
+      exfalso. move: HValid. case; first move=> HValid.
+      by inversion HValid.
+      rewrite csum_included. case; first done.
+      case; by intros (? & ? & ? & ? & ?).
+    }
+    iDestruct "HState" as "#HState". iMod ("HClose" with "[$]") as "HΦ".
+    iModIntro. iMod ("HInvClose" with "[-HΦ]") as "_".
+    { iExists 0, _. iLeft. iFrame "Hpw HTqState". iRight. iFrame.
+      iSplitR; first done. iExists _. iFrame. iPureIntro. lia. }
+    iModIntro. wp_pures. rewrite bool_decide_true; last lia. wp_pures.
+    wp_apply resumeWaiters_spec.
+    { iFrame "HState". iExists _, _, _, _. iSplitR; first done.
+      iFrame "HInv HTq". }
+    by iIntros "_".
+  - iDestruct "Hp" as (n') "[>% Hp]". wp_faa.
+    destruct n=>/=.
+    2: {
+      iDestruct (own_valid_2 with "H● HState")
+        as %[[_ HValid%Some_included]%prod_included _]%auth_both_valid.
+      exfalso. move: HValid. case; first move=> HValid.
+      by inversion HValid.
+      rewrite csum_included. case; first done.
+      case; by intros (? & ? & ? & ? & ?).
+    }
+    iDestruct "HState" as "#HState". iMod ("HClose" with "[$]") as "HΦ".
+    iModIntro. iMod ("HInvClose" with "[-HΦ]") as "_".
+    { iExists 0, _. iRight. iFrame. iSplitR; first done. iExists _. iFrame.
+      iPureIntro. lia. }
+    iModIntro. wp_pures. rewrite bool_decide_true; last lia. wp_pures.
+    wp_apply resumeWaiters_spec.
+    { iFrame "HState". iExists _, _, _, _. iSplitR; first done.
+      iFrame "HInv HTq". }
+    by iIntros "_".
+Qed.
+
+Lemma removeWaiter_local_update γl w r:
+  own γl (● (w, r)) -∗ latch_waiter_registered γl ==∗
+  own γl (● (w - 1, r)).
+Proof.
+  iIntros "H● H◯". iMod (own_update_2 with "H● H◯") as "$"; last done.
+  apply auth_update_dealloc, prod_local_update_1.
+  apply local_update_total_valid=> _ _. rewrite nat_included. move=> Hw.
+  apply nat_local_update. replace ε with 0 by done. lia.
+Qed.
+
+Theorem cancelLatchFuture_spec γl γa γtq γe γd s γf f:
+  is_latch γl γa γtq γe γd s -∗
+  is_latch_future γl γtq γa γf f -∗
+  <<< ▷ thread_queue_future_cancellation_permit γf ∗
+      latch_waiter_permit γl γf >>>
+    cancelLatchFuture array_interface s f @ ⊤ ∖ ↑NFuture ∖ ↑N
+  <<< ∃ (r: bool),
+      if r then future_is_cancelled γf
+      else (∃ v, ▷ future_is_completed γf v) ∗
+           thread_queue_future_cancellation_permit γf ∗
+           latch_waiter_permit γl γf, RET #r >>>.
+Proof.
+  iIntros "#HLatch #HFuture" (Φ) "AU".
+  iDestruct "HLatch" as (e d p pw ->) "[HInv HTq]". wp_lam. wp_pures. wp_lam.
+  wp_pures. awp_apply (try_cancel_thread_queue_future with "HTq HFuture");
+              first by solve_ndisj.
+  iApply (aacc_aupd_commit with "AU"). by solve_ndisj.
+  iIntros "[HCancPermit HWaiter]". iAaccIntro with "HCancPermit".
+  by iIntros "$ !>"; iFrame; iIntros "$ !>".
+  iIntros (r) "Hr". iExists r. destruct r.
+  2: { iDestruct "Hr" as "[$ $]". iFrame. iIntros "!> HΦ !>". by wp_pures. }
+  iDestruct "Hr" as "[#HFutureCancelled Hr]". iFrame "HFutureCancelled".
+  rewrite /is_latch_future /is_thread_queue_future.
+  iDestruct "Hr" as (i f' s ->) "Hr"=> /=.
+  iDestruct "Hr" as "(#H↦~ & #HTh & HToken)". iIntros "!> HΦ !>". wp_pures.
+  wp_lam. wp_pures. wp_apply derefCellPointer_spec.
+  by iDestruct "HTq" as "(_ & $ & _)". iIntros (ℓ) "#H↦". wp_pures. wp_lam.
+  iDestruct "HWaiter" as "[HWaiter|HContra]".
+  2: {
+    iDestruct "HContra" as (?) "HContra".
+    iDestruct (future_is_completed_not_cancelled
+                 with "HContra HFutureCancelled") as %[].
+  }
+  iLöb as "IHCancAllowed".
+  wp_bind (FAA _ _).
+  iInv "HInv" as (n w) "HOpen" "HInvClose".
+  iDestruct "HOpen" as
+      "[(Hpw & HTqState & HRest)|(Hpw & HTqState & >-> & H● & Hp)]".
+  - wp_faa.
+    iAssert (⌜w > 0⌝)%I as %Hw.
+    { iAssert (∃ x, own γl (● (w, x)))%I with "[HRest]" as (?) "H●".
+      by iDestruct "HRest" as "[(_ & H● & _)|(_ & H● & _)]"; by iExists _.
+      iDestruct (own_valid_2 with "H● HWaiter")
+        as %[[HValid%nat_included _]%prod_included _]%auth_both_valid.
+      iPureIntro. simpl in *. lia.
+    }
+    iMod (register_cancellation with "HTq HToken HTqState")
+        as "[HCancToken HTqState]"; first by solve_ndisj.
+    rewrite bool_decide_false; last lia.
+    iDestruct "HTqState" as "(HTqState & HR & #HInhabited)".
+    iAssert (|==> (⌜n > 0⌝ ∧ own γl (● (w - 1, Some (Cinl (Excl (Pos.of_nat n))))) ∗ p ↦ #n
+     ∨ ⌜n = 0⌝ ∧ own γl (● (w - 1, Some (Cinr None))) ∗ (∃ n' : Z, ⌜(n' ≤ 0)%Z⌝ ∧ p ↦ #n')))%I
+                  with "[HRest HWaiter]" as ">HRest".
+    {
+      iDestruct "HRest" as "[(H1 & H● & H2)|(H1 & H● & H2)]";
+        [iLeft|iRight]; iFrame "H1 H2".
+      all: by iMod (removeWaiter_local_update with "H● HWaiter") as "$".
+    }
+    iMod ("HInvClose" with "[-HΦ HCancToken HR]") as "_".
+    { iExists n, (w - 1). iLeft. iFrame "HTqState".
+      replace (Z.of_nat ((w - 1) * 2)) with (Z.of_nat (w * 2) + (-2))%Z by lia.
+      iFrame "Hpw". iFrame. }
+    iModIntro. wp_pures. wp_lam. wp_pures. rewrite bool_decide_false.
+    2: { case. rewrite Nat2Z.inj_mul Z.rem_mul; lia. }
+    wp_pures. wp_bind (getAndSet.getAndSet _ _).
+    awp_apply (markCancelled_spec with "HTq HInhabited H↦ HCancToken HTh")
+              without "HΦ HR".
+    iAaccIntro with "[//]"; first done. iIntros (v) "Hv"=>/=.
+    iIntros "!> (HΦ & HCancHandle)". wp_pures.
+    iAssert (▷ cell_cancellation_handle _ _ _ _ _ _)%I
+            with "[HCancHandle]" as "HCancHandle"; first done.
+    awp_apply (cancelCell_spec with "[] H↦~") without "Hv HΦ".
+    by iDestruct "HTq" as "(_ & $ & _)".
+    iAaccIntro with "HCancHandle". by iIntros "$".
+    iIntros "#HCancelled !> [Hv HΦ]". wp_pures.
+    iDestruct "Hv" as "[[-> _]|Hv]"; first by wp_pures.
+    iDestruct "Hv" as (x ->) "(#HInhabited' & HAwak & %)"; simplify_eq.
+    wp_pures. wp_apply (resumeLatch_spec with "[$]").
+    iIntros "_". wp_pures. iApply "HΦ".
+  - wp_faa.
+    iAssert (⌜w > 0⌝)%I as %Hw.
+    { iDestruct (own_valid_2 with "H● HWaiter")
+        as %[[HValid%nat_included _]%prod_included _]%auth_both_valid.
+      iPureIntro. simpl in *. lia. }
+    iMod (register_cancellation with "HTq HToken HTqState")
+        as "[HCancToken HState]"; first by solve_ndisj.
+    iDestruct "HState" as "(HTqState & HR & #HInhabited)".
+    iMod (removeWaiter_local_update with "H● HWaiter") as "H●".
+    iMod ("HInvClose" with "[-HΦ HCancToken HR]") as "_".
+    { iExists 0, (w - 1). iRight. iFrame.
+      replace ((w * 2 + 1)%nat + -2)%Z with (Z.of_nat ((w - 1) * 2 + 1)) by lia.
+      by iFrame.
+    }
+    iModIntro. wp_pures. wp_lam. wp_pures.
+    rewrite bool_decide_true.
+    2: { congr LitV.
+         rewrite Nat.add_comm Nat2Z.inj_add Nat2Z.inj_mul Z.rem_add //; lia. }
+    wp_pures. wp_bind (getAndSet.getAndSet _ _).
+    awp_apply (markRefused_spec with "HTq HInhabited H↦ HCancToken HTh [//]")
+              without "HΦ HR".
+    iAaccIntro with "[//]"; first done. iIntros (v) "Hv"=>/=.
+    iIntros "!> [HΦ HR]". iDestruct "Hv" as "[[-> _]|Hv]"; first by wp_pures.
+    iDestruct "Hv" as (? ->) "[_ >%]". simplify_eq. wp_pures.
+    iApply "HΦ".
+Qed.
+
+End proof.
