formal-proofs/theories/lib/util/forRange.v
@@ -1,0 +1,69 @@
+From iris.proofmode Require Import tactics.
+From iris.program_logic Require Export atomic.
+From iris.heap_lang Require Import proofmode notation lang.
+From SegmentQueue.util Require Import everything.
+
+Definition forRange : val :=
+  rec: "loop" "n" "fn" :=
+    if: "n" ≤ #0
+    then #()
+    else "loop" ("n"-#1) "fn" ;; "fn" ("n"-#1).
+
+Section for_proof.
+
+Context `{!heapG Σ}.
+
+Theorem forRange_spec (Φ: nat -> iProp Σ) (e: val) (n: nat):
+  (∀ i, ⌜(i < n)%nat⌝ -∗ {{{ Φ i }}}
+                           e #i
+                         {{{ v, RET v; Φ (S i) }}})
+   -∗
+   {{{ Φ O }}}
+     forRange #n e
+   {{{ v, RET v; Φ n }}}.
+Proof.
+  iIntros "#HE" (Ψ).
+  iInduction n as [|n'] "IH" forall (Ψ); iIntros "!> HΦ0 HΨ"; wp_lam; wp_pures.
+  by iApply "HΨ".
+  replace #(S n' - 1) with #n'; last by congr (fun x => LitV (LitInt x)); lia.
+  wp_bind (forRange _ _).
+  wp_apply ("IH" with "[] HΦ0").
+  { iIntros "!>" (i HLt). iApply "HE". iPureIntro. lia. }
+  iIntros (v) "HΦn".
+  wp_pures.
+  replace #(S n' - 1) with #n'; last by congr (fun x => LitV (LitInt x)); lia.
+  wp_apply ("HE" with "[] HΦn"); last done.
+  iPureIntro. lia.
+Qed.
+
+Theorem forRange_resource_map (Φ Ψ: nat -> iProp Σ) (e: val):
+  (∀ (i: nat), {{{ Φ i }}}
+                 e #i
+                 {{{ v, RET v; Ψ i }}})
+    -∗
+  (∀ n, {{{ [∗ list] i ∈ seq 0 n, Φ i }}}
+          forRange #n e
+        {{{ v, RET v; [∗ list] i ∈ seq 0 n, Ψ i }}}).
+Proof.
+  iIntros "#HE" (n Ξ) "!> HΦ HΨ".
+  iApply (forRange_spec
+            (fun j => ([∗ list] i ∈ seq j (n-j), Φ i) ∗
+                   ([∗ list] i ∈ seq 0 j, Ψ i))%I
+            with "[] [HΦ]").
+  - iIntros (i HLt). iIntros "!>" (?) "HPre HPost".
+    replace (seq 0 (S i)) with (seq 0 (i + 1)) by (congr (seq 0); lia).
+    rewrite seq_add /=.
+    destruct (n - i)%nat as [|ni] eqn:X; first by lia.
+    simpl.
+    iDestruct "HPre" as "[[HΦi HΦ] HΨ]".
+    wp_apply ("HE" with "HΦi").
+    iIntros (v) "HΨi".
+    iApply "HPost".
+    replace (n - S i)%nat with ni by lia. iFrame. done.
+  - rewrite Nat.sub_0_r. simpl. iFrame.
+  - iIntros (v) "!> HH".
+    iApply "HΨ".
+    iDestruct "HH" as "[_ $]".
+Qed.
+
+End for_proof.
