formal-proofs/theories/lib/util/getAndUpdate.v
@@ -1,0 +1,13 @@
+From iris.proofmode Require Import tactics.
+From iris.program_logic Require Export atomic.
+From iris.heap_lang Require Import proofmode notation lang.
+
+Definition getAndUpdate : val :=
+  rec: "getAndUpdate" "l" "f" :=
+    let: "o" := ! "l" in
+    match: "f" "o" with
+      NONE => NONE
+    | SOME "v" => if: CAS "l" "o" "v"
+                  then SOME "o"
+                  else "getAndUpdate" "l" "f"
+    end.
